pulse/ulib/experimental/Steel.Semantics.Instantiate.fst
@@ -1,0 +1,38 @@
+module Steel.Semantics.Instantiate
+
+friend Steel.Memory
+
+#set-options "--z3rlimit 20"
+
+let lemma_symmetry () = ()
+let lemma_transitive () = ()
+let lemma_interp_extensionality () = ()
+let lemma_interp_depends_only () = ()
+
+let lemma_associative () = ()
+let lemma_commutative () = ()
+
+let lemma_is_unit () =
+  let lem (y:hprop) : Lemma (star emp y `equals` y /\ star y emp `equals` y)
+    = emp_unit y; star_commutative emp y
+  in
+  Classical.forall_intro lem
+
+let lemma_equals_ext () = ()
+
+let lemma_affine () = ()
+let lemma_emp_valid () = ()
+
+let lemma_disjoint_sym () = ()
+let lemma_disjoint_join () = ()
+
+let lemma_join_commutative () = ()
+let lemma_join_associative () = ()
+
+let lemma_weaken_depends_only_on () = ()
+let lemma_refine_equiv () = ()
+let lemma_refine_star () = ()
+
+let lemma_m_implies_disjoint () = ()
+let lemma_mem_valid_locks_invariant () = ()
+let lemma_valid_upd_heap () = ()
